subtyping examples

plf/Sub.v
@@ -89,4 +89,215 @@ forall T,
 
 (*
 empty |-- (\p:T*Top. p.fst) ((\z:A.z), unit) \in A->A
+
+A -> A, Top
 *)
+
+(*
+
+empty |-- (\p:(A->A * B->B). p) ((\z:A.z), (\z:B.z)) \in T
+
+(A->A * B->B), Top
+*)
+
+(*
+  a:A |-- (\p:(A*T). (p.snd) (p.fst)) (a, \z:A.z) \in A
+  A->A, Top
+*)
+
+(*
+exists S,
+         empty |-- (\p:(A*T). (p.snd) (p.fst)) \in S
+A->A->(A->A), Top
+*)
+
+(*
+exists S t,
+        empty |-- (\x:T. x x) t \in S
+*)
+
+Module STLCSub.
+Inductive ty : Type :=
+  | Ty_Top : ty
+  | Ty_Bool : ty
+  | Ty_Base : string -> ty
+  | Ty_Arrow : ty -> ty -> ty
+  | Ty_Unit : ty
+  | Ty_Prod : ty -> ty -> ty
+.
+
+Inductive tm : Type :=
+  | tm_var : string -> tm
+  | tm_app : tm -> tm -> tm
+  | tm_abs : string -> ty -> tm -> tm
+  | tm_true : tm
+  | tm_false : tm
+  | tm_if : tm -> tm -> tm -> tm
+  | tm_unit : tm
+  | tm_pair : tm -> tm -> tm
+  | tm_fst : tm -> tm
+  | tm_snd : tm -> tm
+.
+
+Declare Custom Entry stlc.
+Notation "<{ e }>" := e (e custom stlc at level 99).
+Notation "( x )" := x (in custom stlc, x at level 99).
+Notation "x" := x (in custom stlc at level 0, x constr at level 0).
+Notation "S -> T" := (Ty_Arrow S T) (in custom stlc at level 50, right associativity).
+Notation "x y" := (tm_app x y) (in custom stlc at level 1, left associativity).
+Notation "\ x : t , y" :=
+  (tm_abs x t y) (in custom stlc at level 90, x at level 99,
+                     t custom stlc at level 99,
+                     y custom stlc at level 99,
+                     left associativity).
+Coercion tm_var : string >-> tm.
+Notation "'Bool'" := Ty_Bool (in custom stlc at level 0).
+Notation "'if' x 'then' y 'else' z" :=
+  (tm_if x y z) (in custom stlc at level 89,
+                    x custom stlc at level 99,
+                    y custom stlc at level 99,
+                    z custom stlc at level 99,
+                    left associativity).
+Notation "'true'" := true (at level 1).
+Notation "'true'" := tm_true (in custom stlc at level 0).
+Notation "'false'" := false (at level 1).
+Notation "'false'" := tm_false (in custom stlc at level 0).
+Notation "'Unit'" :=
+  (Ty_Unit) (in custom stlc at level 0).
+Notation "'unit'" := tm_unit (in custom stlc at level 0).
+Notation "'Base' x" := (Ty_Base x) (in custom stlc at level 0).
+Notation "'Top'" := (Ty_Top) (in custom stlc at level 0).
+Notation "X * Y" :=
+  (Ty_Prod X Y) (in custom stlc at level 2, X custom stlc, Y custom stlc at level 0).
+Notation "( x ',' y )" := (tm_pair x y) (in custom stlc at level 0,
+                                                x custom stlc at level 99,
+                                                y custom stlc at level 99).
+Notation "t '.fst'" := (tm_fst t) (in custom stlc at level 1).
+Notation "t '.snd'" := (tm_snd t) (in custom stlc at level 1).
+Notation "{ x }" := x (in custom stlc at level 1, x constr).
+
+Reserved Notation "'[' x ':=' s ']' t" (in custom stlc at level 20, x constr).
+Fixpoint subst (x : string) (s : tm) (t : tm) : tm :=
+  match t with
+  | tm_var y =>
+      if String.eqb x y then s else t
+  | <{\y:T, t1}> =>
+      if String.eqb x y then t else <{\y:T, [x:=s] t1}>
+  | <{t1 t2}> =>
+      <{([x:=s] t1) ([x:=s] t2)}>
+  | <{true}> =>
+      <{true}>
+  | <{false}> =>
+      <{false}>
+  | <{if t1 then t2 else t3}> =>
+      <{if ([x:=s] t1) then ([x:=s] t2) else ([x:=s] t3)}>
+  | <{unit}> =>
+      <{unit}>
+  | <{ (t1, t2) }> =>
+      <{( [x:=s] t1, [x:=s] t2 )}>
+  | <{t0.fst}> =>
+      <{ ([x:=s] t0).fst}>
+  | <{t0.snd}> =>
+      <{ ([x:=s] t0).snd}>
+  end
+where "'[' x ':=' s ']' t" := (subst x s t) (in custom stlc).
+
+Inductive value : tm -> Prop :=
+  | v_abs : forall x T2 t1,
+      value <{\x:T2, t1}>
+  | v_true :
+      value <{true}>
+  | v_false :
+      value <{false}>
+  | v_unit :
+      value <{unit}>
+.
+
+Hint Constructors value : core.
+Reserved Notation "t '-->' t'" (at level 40).
+Inductive step : tm -> tm -> Prop :=
+  | ST_AppAbs : forall x T2 t1 v2,
+         value v2 ->
+         <{(\x:T2, t1) v2}> --> <{ [x:=v2]t1 }>
+  | ST_App1 : forall t1 t1' t2,
+         t1 --> t1' ->
+         <{t1 t2}> --> <{t1' t2}>
+  | ST_App2 : forall v1 t2 t2',
+         value v1 ->
+         t2 --> t2' ->
+         <{v1 t2}> --> <{v1 t2'}>
+  | ST_IfTrue : forall t1 t2,
+      <{if true then t1 else t2}> --> t1
+  | ST_IfFalse : forall t1 t2,
+      <{if false then t1 else t2}> --> t2
+  | ST_If : forall t1 t1' t2 t3,
+      t1 --> t1' ->
+      <{if t1 then t2 else t3}> --> <{if t1' then t2 else t3}>
+where "t '-->' t'" := (step t t').
+Hint Constructors step : core.
+
+Reserved Notation "T '<:' U" (at level 40).
+Inductive subtype : ty -> ty -> Prop :=
+  | S_Refl : forall T,
+      T <: T
+  | S_Trans : forall S U T,
+      S <: U ->
+      U <: T ->
+      S <: T
+  | S_Top : forall S,
+      S <: <{Top}>
+  | S_Arrow : forall S1 S2 T1 T2,
+      T1 <: S1 ->
+      S2 <: T2 ->
+      <{S1->S2}> <: <{T1->T2}>
+  | S_Prod : forall S1 S2 T1 T2,
+      S1 <: T1 ->
+      S2 <: T2 ->
+      <{S1 * S2}> <: <{T1 * T2}>
+where "T '<:' U" := (subtype T U).
+
+Hint Constructors subtype : core.
+Module Examples.
+Open Scope string_scope.
+Notation x := "x".
+Notation y := "y".
+Notation z := "z".
+Notation A := <{Base "A"}>.
+Notation B := <{Base "B"}>.
+Notation C := <{Base "C"}>.
+Notation String := <{Base "String"}>.
+Notation Float := <{Base "Float"}>.
+Notation Integer := <{Base "Integer"}>.
+Example subtyping_example_0 :
+  <{C->Bool}> <: <{C->Top}>.
+Proof. auto. Qed.
+
+Definition Person : ty :=
+  <{ (String * Top) }>.
+  Definition Student : ty :=
+  <{ (String * Float) }>.
+  Definition Employee : ty :=
+  <{ (String * Integer) }>.
+(* Now use the definition of the subtype relation to prove the following: *)
+Example sub_student_person :
+  Student <: Person.
+Proof. unfold Student. unfold Person. auto. Qed.
+Example sub_employee_person :
+  Employee <: Person.
+Proof. unfold Employee. unfold Person. auto. Qed.
+
+Example subtyping_example_1 :
+  <{Top->Student}> <: <{(C->C)->Person}>.
+Proof with eauto.
+  unfold Student, Person.
+  auto.
+Qed.
+
+Example subtyping_example_2 :
+  <{Top->Person}> <: <{Person->Top}>.
+  Proof with eauto.
+  unfold Student, Person.
+  auto.
+Qed.
+End Examples.
+
